wip

src/imm/imm_bob.v
@@ -68,12 +68,6 @@ Definition fwbob := sb ⨾ ⦗W∩₁Rel⦘ ∪ ⦗W∩₁Rel⦘ ⨾ (sb ∩ sam
 
 Definition bob := fwbob ∪ ⦗R∩₁Acq⦘ ⨾ sb.
 
-Definition ppo := ⦗R⦘ ⨾ (data ∪ ctrl ∪ addr ⨾ sb^? ∪ rfi ∪
-                              rmw ;; ((sb ∩ same_loc) ⨾ ⦗W⦘)^? ∪ rmw_dep ;; sb^?)⁺ ⨾ ⦗W⦘.
-
-Definition ar_int := bob ∪ ppo ∪ detour ∪ ⦗W_ex_acq⦘ ⨾ sb ⨾ ⦗W⦘ 
-                     ∪ ⦗W_ex⦘ ⨾ rfi ⨾ ⦗R∩₁Acq⦘.
-
 Implicit Type WF : Wf G.
 Implicit Type COMP : complete G.
 
@@ -143,60 +137,6 @@ Proof.
 unfold bob; rewrite fwbob_in_sb; basic_solver.
 Qed.
 
-Lemma ppo_in_sb WF: ppo ⊆ sb.
-Proof.
-unfold ppo.
-rewrite (addr_in_sb WF), (data_in_sb WF), (ctrl_in_sb WF).
-rewrite (rmw_dep_in_sb WF).
-arewrite (rfi ⊆ sb).
-rewrite WF.(rmw_in_sb).
-rewrite inclusion_seq_eqv_l, inclusion_seq_eqv_r.
-assert (sb⁺ ⊆ sb) as AA.
-{ generalize (@sb_trans G). ins. relsf. }
-etransitivity.
-2: by apply AA.
-apply clos_trans_mori.
-generalize (@sb_trans G); ins; relsf.
-generalize (@sb_trans G). basic_solver 10.
-Qed.
-
-Lemma rmw_in_ppo WF : rmw ⊆ ppo.
-Proof.
-unfold ppo; rewrite (wf_rmwD WF) at 1.
-rewrite R_ex_in_R at 1.
-rewrite <- ct_step.
-basic_solver 10.
-Qed.
-
-(* Lemma rmw_sb_W_in_ppo WF : rmw ⨾ sb ⨾ ⦗W⦘ ⊆ ppo. *)
-(* Proof. *)
-(* unfold ppo; rewrite (wf_rmwD WF). *)
-(* rewrite (dom_l (wf_rmwD WF)), R_ex_in_R at 1. *)
-(* rewrite (rmw_in_sb WF) at 1. *)
-(* rewrite <- ct_step. *)
-(* generalize (@sb_trans G). *)
-(* basic_solver 12. *)
-(* Qed. *)
-
-Lemma data_in_ppo WF : data ⊆ ppo.
-Proof.
-unfold ppo; rewrite (wf_dataD WF) at 1.
-hahn_frame; econs; basic_solver 12.
-Qed.
-
-(* Lemma R_ex_sb_in_ppo WF : ⦗R_ex⦘ ⨾ sb ⨾ ⦗W⦘ ⊆ ppo. *)
-(* Proof. *)
-(*   arewrite (⦗R_ex⦘ ⊆ ⦗R⦘ ;; ⦗R_ex⦘) by type_solver. *)
-(*   unfold ppo. hahn_frame. rewrite <- ct_step. eauto with hahn. *)
-(* Qed. *)
-
-(* Lemma rmw_sb_cr_W_in_ppo WF : rmw ⨾ sb^? ⨾ ⦗W⦘ ⊆ ppo. *)
-(* Proof. *)
-(*   rewrite crE. rewrite seq_union_l, seq_union_r, seq_id_l. *)
-(*   rewrite WF.(rmw_sb_W_in_ppo). *)
-(*   rewrite WF.(rmw_in_ppo). eauto with hahn hahn_full. *)
-(* Qed. *)
-
 
 (******************************************************************************)
 (** ** Relations in graph *)
@@ -218,43 +158,10 @@ rewrite (wf_fwbobE WF), wf_sbE.
 basic_solver 42.
 Qed.
 
-Lemma wf_ppoE WF : ppo ≡ ⦗E⦘ ⨾ ppo ⨾ ⦗E⦘.
-Proof.
-split; [|basic_solver].
-unfold ppo.
-rewrite !seqA, seq_eqvC.
-hahn_frame.
-seq_rewrite seq_eqvC.
-rewrite !seqA.
-hahn_frame.
-rewrite <- inclusion_ct_seq_eqv_r, <- inclusion_ct_seq_eqv_l.
-apply inclusion_t_t.
-unfold Execution.rfi.
-rewrite (wf_rfE WF), (wf_dataE WF), (wf_rmw_depE WF) at 1.
-rewrite (wf_addrE WF), (wf_ctrlE WF), (wf_rmwE WF) at 1.
-rewrite wf_sbE at 1 2 3 4.
-basic_solver 21.
-Qed.
-
-Lemma wf_ar_intE WF : ar_int ≡ ⦗E⦘ ⨾ ar_int ⨾ ⦗E⦘.
-Proof.
-split; [|basic_solver].
-unfold ar_int.
-rewrite (wf_bobE WF), (wf_ppoE WF) at 1.
-rewrite (wf_detourE WF), (@wf_sbE G), (wf_rfiE WF).
-basic_solver 42.
-Qed.
-
 
 (******************************************************************************)
 (** ** more properties  *)
 (******************************************************************************)
-
-Lemma wf_ppoD: ppo ≡ ⦗R⦘ ⨾ ppo ⨾ ⦗W⦘.
-Proof.
-split; [|basic_solver].
-unfold ppo; basic_solver.
-Qed.
 
 Lemma fwbob_r_sb: fwbob ⨾ ⦗ R ⦘ ⨾ sb ⊆ fwbob.
 Proof.
@@ -267,117 +174,6 @@ Lemma bob_r_sb: bob ⨾ ⦗ R ⦘ ⨾ sb ⊆ bob.
 Proof.
 unfold bob; relsf; rewrite fwbob_r_sb.
 generalize (@sb_trans G); basic_solver 21.
-Qed.
-
-Lemma fwbob_ppo WF: fwbob ⨾ ppo ⊆ fwbob.
-Proof.
-rewrite wf_ppoD, (ppo_in_sb WF).
-sin_rewrite fwbob_r_sb.
-basic_solver.
-Qed.
-
-Lemma bob_ppo WF: bob ⨾ ppo ⊆ bob.
-Proof.
-rewrite wf_ppoD, (ppo_in_sb WF).
-sin_rewrite bob_r_sb.
-basic_solver.
-Qed.
-
-Lemma ar_int_in_sb WF: ar_int ⊆ sb.
-Proof.
-unfold ar_int.
-rewrite bob_in_sb.
-rewrite (ppo_in_sb WF).
-arewrite (detour ⊆ sb).
-arewrite (rfi ⊆ sb).
-basic_solver 21.
-Qed.
-
-Lemma ppo_rfi_ppo : ppo ⨾ rfi ⨾ ppo ⊆ ppo.
-Proof.
-unfold ppo.
-rewrite !seqA.
-arewrite_id ⦗W⦘ at 2.
-arewrite_id ⦗R⦘ at 2.
-arewrite (rfi ⊆ (data ∪ ctrl ∪ addr ⨾ sb^? ∪ rfi ∪ rmw ⨾ (sb ∩ same_loc ⨾ ⦗W⦘)^? ∪ rmw_dep ⨾ sb^?)＊) at 2.
-rewrite inclusion_t_rt at 1.
-relsf.
-Qed.
-
-Lemma deps_rfi_in_ppo : ⦗R⦘ ⨾ (deps ∪ rfi)⁺ ⨾ ⦗W⦘ ⊆ ppo.
-Proof.
-  unfold ppo, Execution.deps.
-  hahn_frame.
-  apply inclusion_t_t; basic_solver 21.
-Qed.
-
-(* Lemma ppo_alt WF  *)
-(*   (RMW_DEPS : rmw ⊆ deps) *)
-(*   (DEPS_RMW_FAIL : rmw_dep ⨾ sb ⊆ ctrl) :  *)
-(*   ppo ≡ ⦗R⦘ ⨾ (data ∪ ctrl ∪ addr ⨾ sb^? ∪ rfi)⁺ ⨾ ⦗W⦘. *)
-(* Proof. *)
-(*   unfold ppo. *)
-(* Admitted. *)
-
-(* generalize (@sb_trans G); ins. *)
-(* unfold ppo. *)
-(* split. *)
-(* 2: by hahn_frame; apply inclusion_t_t; basic_solver 12. *)
-(* rewrite RMW_DEPS; unfold Execution.deps. *)
-(* rewrite path_ut_first; relsf; unionL. *)
-(* by hahn_frame; apply inclusion_t_t; basic_solver 12. *)
-(* arewrite ((data ∪ ctrl ∪ addr ⨾ sb^? ∪ rfi ∪ (data ∪ addr ∪ ctrl) ∪ rmw_dep ⨾ sb^?) ⊆ sb). *)
-(* { rewrite (data_in_sb WF), (addr_in_sb WF), (ctrl_in_sb WF). *)
-(*   arewrite (rfi ⊆ sb). *)
-(*   rewrite (rmw_dep_in_sb WF). *)
-(*   relsf. } *)
-(* relsf. *)
-(* rewrite (dom_r (wf_rmw_depD WF)), !seqA. *)
-(* rewrite (crE sb) at 2; relsf; unionL. *)
-(* by rewrite R_ex_in_R; type_solver. *)
-(* hahn_frame. *)
-(* sin_rewrite RMW_CTRL_FAIL. *)
-(* rewrite DEPS_RMW_FAIL. *)
-(* rewrite ct_end. *)
-(* apply inclusion_seq_mon; [apply inclusion_rt_rt|]; basic_solver 42. *)
-(* Qed. *)
-
-Lemma bob_in_ar_int : bob ⊆ ar_int.
-Proof. unfold ar_int. basic_solver 10. Qed.
-
-Lemma ppo_in_ar_int : ppo ⊆ ar_int.
-Proof. unfold ar_int. basic_solver 10. Qed.
-
-Lemma detour_in_ar_int : detour ⊆ ar_int.
-Proof. unfold ar_int. basic_solver. Qed.
-
-Lemma w_ex_acq_sb_w_in_ar_int : ⦗W_ex_acq⦘ ⨾ sb ⨾ ⦗W⦘ ⊆ ar_int.
-Proof. unfold ar_int. basic_solver 10. Qed.
-
-Lemma bob_ppo_W_sb WF :
-  (bob ∪ ppo ∪ ⦗W_ex_acq⦘ ⨾ sb ⨾ ⦗W⦘)⁺ ⊆ ppo ∪ ppo ^? ;; (bob ∪ ⦗W_ex_acq⦘ ⨾ sb ⨾ ⦗W⦘)^+.
-Proof.
-arewrite (bob ∪ ppo ∪ ⦗W_ex_acq⦘ ⨾ sb ⨾ ⦗W⦘ ⊆
-         (bob ∪ ⦗W_ex_acq⦘ ⨾ sb ⨾ ⦗W⦘) ∪ ppo).
-basic_solver 12.
-apply ct_ind_left with (P:= fun r =>  r).
-by auto with hahn.
-- arewrite(bob ⊆ (bob ∪ ⦗W_ex_acq⦘ ⨾ sb ⨾ ⦗W⦘)⁺).
-  arewrite(⦗W_ex_acq⦘ ⨾ sb ⨾ ⦗W⦘ ⊆ (bob ∪ ⦗W_ex_acq⦘ ⨾ sb ⨾ ⦗W⦘)⁺) at 2.
-  basic_solver 12.
-- intros k H. rewrite H; clear k H; rewrite crE; relsf; unionL.
-+ rewrite (bob_ppo WF). 
-  arewrite(bob ⊆ (bob ∪ ⦗W_ex_acq⦘ ⨾ sb ⨾ ⦗W⦘)⁺).
-  basic_solver.
-+ rewrite (wf_ppoD) at 1. type_solver.
-+ rewrite (wf_ppoD) at 1 2. type_solver.
-+ arewrite(bob ⊆ (bob ∪ ⦗W_ex_acq⦘ ⨾ sb ⨾ ⦗W⦘)^*); relsf.
-+ sin_rewrite (bob_ppo WF). 
-  arewrite(bob ⊆ (bob ∪ ⦗W_ex_acq⦘ ⨾ sb ⨾ ⦗W⦘)^*); relsf.
-+ arewrite(⦗W_ex_acq⦘ ⨾ sb ⨾ ⦗W⦘ ⊆ (bob ∪ ⦗W_ex_acq⦘ ⨾ sb ⨾ ⦗W⦘)^*) at 1; relsf.
-+ rewrite (wf_ppoD) at 1. type_solver.
-+ basic_solver 12.
-+ rewrite (wf_ppoD) at 1 2. type_solver.
 Qed.
 
 Lemma bob_sb :
@@ -416,6 +212,5 @@ relsf; unionL.
   by arewrite (fwbob ⊆ fwbob^+); basic_solver 21.
 - generalize (@sb_trans G); basic_solver 12.
 Qed.
-
 
 End IMM.
