src/hardware/immToARM.v
@@ -7,7 +7,8 @@ Require Import Events.
 Require Import Execution.
 Require Import Execution_eco.
 Require Import Arm.
-Require Import imm_common.
+Require Import imm_bob.
+Require Import imm_ppo.
 Require Import imm_hb.
 Require Import imm.
 
