src/imm/Rel_opt.v
@@ -6,7 +6,8 @@ Require Import Classical Peano_dec.
 From hahn Require Import Hahn.
 
 Require Import Events Execution Execution_eco.
-Require Import imm_common.
+Require Import imm_bob.
+Require Import imm_ppo.
 Require Import imm_hb.
 Require Import imm.
 
@@ -186,8 +187,6 @@ Lemma F_eq : F' ≡₁ F.
 Proof. unfold G', relax_release_labels; type_solver 22. Qed.
 Lemma W_eq : W' ≡₁ W.
 Proof. unfold G', relax_release_labels; type_solver 22. Qed.
-Lemma W_ex_eq : W_ex' ≡₁ W_ex.
-Proof. unfold G', relax_release_labels; type_solver 22. Qed.
 Lemma W_ex_acq_eq : W_ex_acq' ≡₁ W_ex_acq.
 Proof. unfold G', relax_release_labels.
 unfold Execution.W_ex; mode_unfolder; ins; unfold xmod; basic_solver 22. Qed.
@@ -277,7 +276,7 @@ Proof. by unfold G'; ins. Qed.
 
 Lemma bob_eq : bob ⊆ bob'⁺ ∪ rmw' ∪ ⦗W ∩₁ Rel⦘ ⨾ sb' ∩ same_loc' ⨾ ⦗W'⦘.
 Proof.
-unfold imm_common.bob, imm_common.fwbob.
+unfold imm_bob.bob, imm_bob.fwbob.
 rewrite F_eq, R_eq, W_eq, Rel_eq, sb_eq, F_AcqRel_eq, R_Acq_eq, same_loc_eq.
 unionL.
 - rewrite W_REL; unionL.
@@ -296,9 +295,8 @@ Qed.
 
 Lemma ppo_eq: ppo' ≡ ppo.
 Proof.
-unfold imm_common.ppo, Execution.rfi.
-rewrite W_eq, R_eq, sb_eq, data_eq, addr_eq, ctrl_eq, rf_eq, rmw_eq, same_loc_eq.
-done.
+unfold imm_ppo.ppo, Execution.rfi.
+by rewrite W_eq, R_eq, sb_eq, data_eq, addr_eq, ctrl_eq, rf_eq, R_ex_eq.
 Qed.
 
 Lemma detour_eq: detour' ≡ detour.
@@ -593,23 +591,17 @@ rewrite bob_eq.
 rewrite <- sb_eq.
 rewrite <- W_ex_acq_eq.
 rewrite <- W_eq at 2.
-rewrite <- rfi_eq.
-rewrite <- W_ex_eq.
-rewrite <- R_Acq_eq.
-rewrite <- R_eq.
 
 rewrite (rmw_in_ppo WFp) at 1.
 
-apply acyclic_mon with (r:= psc' ∪ ppo' ∪ rfe' ∪ detour' 
- ∪ ⦗W_ex_acq'⦘ ⨾ sb' ⨾ ⦗W'⦘ ∪ ⦗W_ex'⦘ ⨾ rfi' ⨾ ⦗R' ∩₁ Acq'⦘ 
- ∪ bob'⁺ ∪ ⦗W ∩₁ Rel⦘ ⨾ sb' ∩ same_loc' ⨾ ⦗W'⦘).
-2: basic_solver 30.
+apply acyclic_mon with (r:= psc' ∪ ppo' ∪ rfe' ∪ detour' ∪ ⦗W_ex_acq'⦘ ⨾ sb' ⨾ ⦗W'⦘ ∪ bob'⁺ ∪ ⦗W ∩₁ Rel⦘ ⨾ sb' ∩ same_loc' ⨾ ⦗W'⦘).
+2: basic_solver 20.
 apply acyclic_union1.
 -
 
 red.
 rewrite ct_of_union_ct_r; eapply acyclic_mon; [edone|].
-basic_solver 21.
+basic_solver 12.
 -
 apply acyclic_mon with (r:=sb').
 red; generalize (@sb_trans G'); ins; relsf; apply (@sb_irr G').
@@ -617,17 +609,16 @@ basic_solver.
 -
 
 
-(* arewrite (sb' ∩ same_loc' ⊆ sb'). *)
+arewrite (sb' ∩ same_loc' ⊆ sb').
 
-assert (transitive (⦗W ∩₁ Rel⦘ ⨾ sb' ∩ same_loc' ⨾ ⦗W'⦘)).
+assert (transitive (⦗W ∩₁ Rel⦘ ⨾ sb' ⨾ ⦗W'⦘)).
 {
 apply transitiveI; rewrite !seqA.
 arewrite_id (⦗W'⦘ ⨾ ⦗W ∩₁ Rel⦘).
 basic_solver.
 relsf.
-arewrite (sb' ∩ same_loc' ⨾ sb' ∩ same_loc' ⊆ sb' ∩ same_loc').
-generalize (@sb_trans G') (@same_loc_trans _ lab').
-basic_solver 21.
+arewrite (sb' ⨾ sb' ⊆ sb').
+apply transitiveI, (@sb_trans G').
 done.
 }
 
@@ -637,9 +628,7 @@ rewrite ct_of_union_ct_r.
 
 
 rewrite ct_end, !seqA.
-arewrite ((psc' ∪ ppo' ∪ rfe' ∪ detour' ∪ 
-  ⦗W_ex_acq'⦘ ⨾ sb' ⨾ ⦗W'⦘ ∪ 
-  ⦗W_ex'⦘ ⨾ rfi' ⨾ ⦗R' ∩₁ Acq'⦘ ∪ bob') ⨾ ⦗W ∩₁ Rel⦘ ⊆ sb' ⨾ ⦗W ∩₁ Rel⦘).
+arewrite ((psc' ∪ ppo' ∪ rfe' ∪ detour' ∪ ⦗W_ex_acq'⦘ ⨾ sb' ⨾ ⦗W'⦘ ∪ bob') ⨾ ⦗W ∩₁ Rel⦘ ⊆ sb' ⨾ ⦗W ∩₁ Rel⦘).
 {
 relsf; unionL.
 - rewrite (dom_r (@wf_pscD G')).
@@ -649,7 +638,6 @@ rewrite F_Sc_eq; type_solver 21.
 rewrite R_eq; type_solver 21.
 - by rewrite detour_in_sb.
 - by basic_solver.
-- unfold Execution.rfi; basic_solver.
 - by rewrite bob_in_sb.
 }
 
@@ -661,18 +649,16 @@ rewrite <- sb_eq, <- rmw_eq.
 arewrite (⦗F ∩₁ Rel⦘ ⊆ ⦗F ∩₁ Acq/Rel⦘) by mode_solver.
 rewrite <- F_AcqRel_eq, <- F_eq.
 
-arewrite ((sb'^? ⨾ ⦗F' ∩₁ Acq/Rel'⦘ ⨾ sb' ∪ rmw') ⨾ sb' ∩ same_loc' ⨾ ⦗W'⦘ 
- ⊆ (psc' ∪ ppo' ∪ rfe' ∪ detour' 
-     ∪ ⦗W_ex_acq'⦘ ⨾ sb' ⨾ ⦗W'⦘ ∪ ⦗W_ex'⦘ ⨾ rfi' ⨾ ⦗R' ∩₁ Acq'⦘ ∪ bob')⁺).
+arewrite ((sb'^? ⨾ ⦗F' ∩₁ Acq/Rel'⦘ ⨾ sb' ∪ rmw') ⨾ sb' ⨾ ⦗W'⦘ ⊆ (psc' ∪ ppo' ∪ rfe' ∪ detour' ∪ ⦗W_ex_acq'⦘ ⨾ sb' ⨾ ⦗W'⦘ ∪ bob')⁺).
 {
 
 relsf; unionL.
 
 -
 rewrite !seqA.
-arewrite (sb' ⨾ sb' ∩ same_loc' ⨾ ⦗W'⦘ ⊆ sb').
+arewrite (sb' ⨾ sb' ⨾ ⦗W'⦘ ⊆ sb').
 by generalize (@sb_trans G'); basic_solver.
-unfold imm_common.bob, imm_common.fwbob.
+unfold imm_bob.bob, imm_bob.fwbob.
 
 case_refl _.
 unfolder; ins; eapply t_step; basic_solver 21.
@@ -680,18 +666,18 @@ unfolder; ins; eapply t_step; basic_solver 21.
 unfolder; ins; desf; eapply t_trans; eapply t_step; basic_solver 21.
 -
 
-arewrite (rmw' ⨾ sb' ∩ same_loc' ⨾ ⦗W'⦘ ⊆ ppo').
-{ unfold imm_common.ppo; rewrite <- ct_step.
+arewrite (rmw' ⨾ sb' ⨾ ⦗W'⦘ ⊆ ppo').
+{ unfold imm_ppo.ppo; rewrite <- ct_step.
 rewrite (dom_l (wf_rmwD WFp)) at 1; rewrite !seqA.
-rewrite (dom_l (wf_rmwD WFp)), R_ex_in_R at 1; rewrite !seqA. 
-basic_solver 21.
+rewrite (dom_l (wf_rmwD WFp)), R_ex_in_R at 1; rewrite !seqA.
+rewrite (rmw_in_sb WFp).
+generalize (@sb_trans G'); basic_solver 21.
 }
 
 by red; ins; eapply t_step; basic_solver 12.
 
 }
 relsf.
-
 
 red; rels.
 eapply acyclic_mon; [edone|basic_solver 12].
