src/imm/imm_common_more.v
@@ -8,7 +8,7 @@ From hahn Require Import Hahn.
 Require Import Events.
 Require Import Execution.
 Require Import Execution_eco.
-Require Import imm_common.
+Require Import imm_ppo.
 
 Set Implicit Arguments.
 Remove Hints plus_n_O.
