src/imm/imm_new_ppo.v
@@ -207,66 +207,21 @@ rewrite (dom_r wf_pscD) at 1; rewrite (dom_l (wf_rfeD WF)); type_solver 12.
 rewrite (dom_r (wf_rfeD WF)) at 1; rewrite (dom_l (wf_rfeD WF)); type_solver 12.
 Qed.
 
-Lemma sw_in_ar_helper_old WF:
-  ((sb ∩ same_loc)^? ⨾ rf ⨾ rmw)＊ ⊆
-  (sb ∩ same_loc ⨾ ⦗W⦘)^? ∪ (sb ∩ same_loc)^? ⨾ (rfe ⨾ rmw ⨾ sb^? ⨾ ⦗W⦘)⁺.
+Lemma sw_in_ar1 WF :
+  sw ⊆ (<|F ∩₁ Rel|> ;; sb ∪ <|W ∩₁ Rel|> ;; (sb ∩ same_loc⨾ ⦗W⦘)^?) ⨾ 
+  (rfe ∪ ar_int)⁺ ⨾ sb^? ∪ sb.
 Proof.
-  rewrite rtE at 1; relsf; unionL; [basic_solver 21|].
-  rewrite rfi_union_rfe; relsf.
-  rewrite path_union.
-  unionL.
-  { rewrite (dom_r (wf_rmwD WF)) at 1.
-    rewrite (rfi_in_sbloc' WF) at 1.
-    rewrite (rmw_in_sb_loc WF) at 1.
-    generalize (@sb_same_loc_trans G); ins; relsf.
-    assert (transitive (sb ∩ same_loc ⨾ ⦗W⦘)).
-    2: by relsf.
-    generalize sb_same_loc_trans; unfold transitive.
+remember (rfe ∪ ar_int) as ax.
+  assert (rmw ⨾ (sb ∩ same_loc)^?⨾ ⦗W⦘ ⊆ ax) as CC.
+  { rewrite crE; relsf; unionL.
+    - rewrite (rmw_in_ppo WF).
+      desf; unfold imm_ppo.ar_int; basic_solver 12.
+    - desf; unfold imm_ppo.ar_int, imm_ppo.ppo.
+    rewrite <- ct_step at 1. rewrite WF.(wf_rmwD) at 1. rewrite R_ex_in_R.
     basic_solver 21. }
-  rewrite ct_seq_swap, !seqA.
-  rewrite (dom_r (wf_rmwD WF)) at 3.
-  rewrite (rfi_in_sbloc' WF) at 1 2.
-  rewrite (rmw_in_sb_loc WF) at 1 3.
-  generalize (@sb_same_loc_trans G); intros HH; relsf.
-  arewrite ((sb ∩ same_loc) ⊆ sb) at 3.
-  unionR right.
-  rewrite (dom_l WF.(wf_rfeD)), !seqA.
-  rewrite <- seqA with (r2:= ⦗W⦘).
-  rewrite ct_rotl, !seqA.
-  arewrite ((sb ∩ same_loc)^? ⨾ (sb ∩ same_loc)^? ⊆ (sb ∩ same_loc)^?).
-  { generalize HH. basic_solver 10. }
-  hahn_frame.
-  arewrite ((sb ⨾ ⦗W⦘)＊ ⨾ (sb ∩ same_loc)^? ⊆ sb^?).
-  { arewrite_id ⦗W⦘. rewrite seq_id_r. rewrite rt_of_trans.
-    2: by apply sb_trans.
-    generalize sb_trans.
-    basic_solver 10. }
-  arewrite (rmw ⨾ (sb ⨾ ⦗W⦘)＊ ⊆ rmw ⨾ sb^? ⨾ ⦗W⦘).
-  2: { rewrite (dom_l WF.(wf_rfeD)) at 1 2; rewrite !seqA.
-       arewrite_id ⦗W⦘ at 1. rewrite seq_id_l.
-       apply ct_end. }
-  rewrite rtE, seq_union_r.
-  unionL.
-  { rewrite (dom_r (wf_rmwD WF)) at 1. basic_solver 10. }
-  rewrite ct_of_trans.
-  { basic_solver 10. }
-  generalize sb_trans. basic_solver.
-Qed.
-
-Lemma sw_in_ar WF :
-  sw ⊆ sb^? ⨾ ⦗W⦘ ⨾ ar⁺ ⨾ (rmw ⨾ sb^?)^? ∪ sb.
-Proof.
-  assert ((sb ⨾ ⦗F⦘)^? ⨾ ⦗Acq⦘ ⊆ ar^?) as BB.
-  { arewrite (⦗Acq⦘ ⊆ ⦗Acq/Rel⦘) by mode_solver.
-      unfold ar, imm_ppo.ar_int, imm_bob.bob, imm_bob.fwbob.
-      basic_solver 21. }
-  assert (rmw ⨾ sb^? ⨾ ⦗W⦘ ⊆ ar) as CC.
-  { unfold ar, imm_ppo.ar_int, imm_ppo.ppo.
-    rewrite <- ct_step, (dom_l (wf_rmwD WF)), (rmw_in_sb WF) at 1.
-    generalize (@sb_trans G) (R_ex_in_R); basic_solver 21. }
-
+(*
   assert (fwbob G ⊆ ar) as EE.
-  { unfold ar. unfold imm_ppo.ar_int.
+  { unfold ar. unfold imm_common.ar_int.
     rewrite fwbob_in_bob. basic_solver 10. }
 
   assert (⦗Rel⦘ ⨾ (⦗F⦘ ⨾ sb)^? ⨾ ⦗W⦘ ⨾ sb ∩ same_loc ⨾ ⦗W⦘ ⊆ sb^? ⨾ ⦗W⦘ ⨾ ar^?) as DD.
@@ -291,101 +246,157 @@ Proof.
 
   assert (ar^? ⨾ ar ⨾ ar^? ⊆ ar⁺) as WW.
   { arewrite (ar ⊆ ar⁺) at 2. by rewrite ct_cr, cr_ct. }
-
+*)
   unfold imm_hb.sw, imm_hb.release, imm_hb.rs.
-  rewrite (sw_in_ar_helper_old WF).
-  
+
+
+  rewrite (sw_in_ar_helper WF).
+
+
   rewrite (dom_l (wf_rfeD WF)).
-  rewrite !seqA, inclusion_ct_seq_eqv_l.
-  arewrite ((sb ∩ same_loc)^? ⨾ ⦗W⦘ ⊆ (sb ∩ same_loc ⨾ ⦗W⦘)^? ⨾ ⦗W⦘).
-  { basic_solver 10. }
-  arewrite (rfe ⊆ ar).
-  arewrite (rfi ⊆ sb).
+  rewrite !seqA. 
 
-  arewrite ((sb ∩ same_loc ⨾ ⦗W⦘)^? ∪ (sb ∩ same_loc ⨾ ⦗W⦘)^? ⨾ ⦗W⦘ ⨾ (ar ⨾ rmw ⨾ sb^? ⨾ ⦗W⦘)⁺ ⊆
-          (sb ∩ same_loc ⨾ ⦗W⦘)^? ⨾ (ar ⨾ rmw ⨾ sb^? ⨾ ⦗W⦘)＊).
-  { basic_solver 10. }
-  arewrite (sb ∩ same_loc ⨾ ⦗W⦘ ∪ (sb ∩ same_loc ⨾ ⦗W⦘)^? ⨾ (ar ⨾ rmw ⨾ sb^? ⨾ ⦗W⦘)＊ ⊆
-               (sb ∩ same_loc ⨾ ⦗W⦘)^? ⨾ (ar ⨾ rmw ⨾ sb^? ⨾ ⦗W⦘)＊).
-  { basic_solver 10. }
+arewrite (rfi ⊆ sb).
+arewrite (rfe ⊆ ax) by desf; basic_solver.
+arewrite (sb ∩ same_loc ⨾ ⦗W⦘
+       ∪ ((sb ∩ same_loc ⨾ ⦗W⦘)^?
+          ∪ (sb ∩ same_loc)^?
+            ⨾ (⦗W⦘ ⨾ ax ⨾ rmw ⨾ (sb ∩ same_loc)^? ⨾ ⦗W⦘)⁺) ⊆
+((sb ∩ same_loc ⨾ ⦗W⦘)^?
+          ∪ (sb ∩ same_loc)^?
+            ⨾ (⦗W⦘ ⨾ ax ⨾ rmw ⨾ (sb ∩ same_loc)^? ⨾ ⦗W⦘)⁺)).
 
-  assert (⦗Rel⦘ ⨾ (⦗F⦘ ⨾ sb)^? ⨾ ⦗W⦘ ⨾ (sb ∩ same_loc ⨾ ⦗W⦘)^? ⊆
-            ⦗Rel⦘ ⨾ (⦗F⦘ ⨾ sb)^? ⨾ ⦗W⦘ ⨾ (sb ∩ same_loc)^? ⨾ ⦗W⦘) as ZZ.
-  { basic_solver 20. }
+relsf; unionL.
+-
+generalize (@sb_trans G).
+basic_solver 21.
+- rewrite !seqA.
+arewrite ( (sb ∩ same_loc ⨾ ⦗W⦘)^?
+      ⨾ (sb ∩ same_loc)^? ⨾ ⦗W⦘ ⊆ (sb ∩ same_loc ⨾ ⦗W⦘)^?).
 
-  assert (rmw ⨾ sb^? ⨾ ⦗W⦘ ⊆ ppo G) as QQ.
-  { rewrite crE, !seq_union_l, !seq_union_r.
-    rewrite rmw_sb_W_in_ppo, rmw_in_ppo; auto.
-    basic_solver. }
+by generalize (@sb_same_loc_trans G); basic_solver 21.
 
-  assert (ar ⨾ ar ⊆ ar⁺) as PP.
-  { arewrite (ar ⊆ ar⁺). apply ct_unit. }
-  
-  rewrite rtE. rewrite !seq_union_l, !seq_union_r, !seq_id_l.
-  unionL.
-  { unionR right. generalize (@sb_trans G). basic_solver 21. }
-  { rewrite !seqA.
-    arewrite ((sb ∩ same_loc ⨾ ⦗W⦘)^? ⨾ (sb ∩ same_loc)^? ⨾ ⦗W⦘ ⊆
-              (sb ∩ same_loc)^? ⨾ ⦗W⦘).
-    { generalize (@sb_same_loc_trans G). basic_solver 10. }
-    sin_rewrite FF. rewrite !seqA.
-    rewrite BB. sin_rewrite WW. basic_solver 10. }
-  { sin_rewrite ZZ. sin_rewrite FF. rewrite !seqA.
-    rewrite ct_end, !seqA.
-    arewrite (rmw ⨾ sb^? ⨾ ⦗W⦘ ⨾ sb ⨾ (sb ⨾ ⦗F⦘)^? ⨾ ⦗Acq⦘ ⊆
-                  rmw ⨾ sb^?).
-    { generalize (@sb_trans G). basic_solver 10. }
-    sin_rewrite QQ. arewrite (ppo G ⊆ ar).
-    arewrite (ar^? ⨾ (ar ⨾ ar)＊ ⨾ ar ⊆ ar⁺).
-    2: basic_solver 20.
-    sin_rewrite PP.
-    rewrite rt_of_ct.
-    rewrite <- ct_end. apply cr_ct. }
-  unionR left.
-  sin_rewrite ZZ. sin_rewrite FF. rewrite !seqA.
-  rewrite ct_end, !seqA. rewrite BB.
-  assert (sb^? ⨾ ⦗W⦘ ⨾ (sb ∩ same_loc)^? ⨾ ⦗W⦘ ⊆ sb^? ⨾ ⦗W⦘) as TT.
-  { generalize (@sb_trans G). basic_solver 10. }
-  sin_rewrite TT.
-  rewrite !seqA.
-  repeat sin_rewrite QQ. arewrite (ppo G ⊆ ar).
-  repeat sin_rewrite PP.
-  rewrite rt_of_ct. sin_rewrite ct_unit. sin_rewrite ct_cr.
-  sin_rewrite rt_ct. sin_rewrite cr_ct. basic_solver 10.
+
+rewrite <- ct_step.
+generalize (@sb_trans G).
+basic_solver 21.
+
+-
+
+rewrite CC.
+rewrite inclusion_ct_seq_eqv_l.
+arewrite ((ax ⨾ ax)⁺ ⊆ ax⁺).
+
+by arewrite (ax ⊆ ax⁺); arewrite (ax ⊆ ax^*) at 2; relsf.
+
+generalize (@sb_trans G).
+basic_solver 21.
+- rewrite ct_end.
+rewrite !seqA.
+arewrite ((sb ∩ same_loc)^?
+                ⨾ ⦗W⦘
+                  ⨾ (sb ∩ same_loc)^? ⊆ (sb ∩ same_loc)^?).
+by generalize (@sb_same_loc_trans G); basic_solver 12.
+rewrite CC.
+sin_rewrite CC.
+
+arewrite (ax ⊆ ax⁺) at 1.
+arewrite (ax ⊆ ax^*) at 2.
+arewrite (ax ⊆ ax⁺) at 3.
+arewrite (ax ⊆ ax^*) at 4.
+arewrite (ax ⊆ ax^*) at 5.
+relsf.
+rewrite rtE; relsf; unionL.
+
+generalize (@sb_trans G).
+basic_solver 21.
+
+
+
+rewrite inclusion_ct_seq_eqv_l.
+rels.
+arewrite ((⦗W⦘ ⨾ ax⁺) ⨾ ⦗W⦘ ⨾ ax⁺ ⊆ ⦗W⦘ ⨾ ax^+).
+{ 
+rewrite !seqA; hahn_frame_l.
+arewrite_id ⦗W⦘.
+rewrite inclusion_t_rt at 1.
+relsf. }
+
+generalize (@sb_trans G).
+basic_solver 21.
+
 Qed.
 
-Lemma f_sc_hb_f_sc_in_ar WF : 
-  ⦗F ∩₁ Sc⦘ ⨾ hb ⨾ ⦗F ∩₁ Sc⦘ ⊆ ar⁺.
+Lemma sw_in_ar WF :
+  sw ⊆ (rfe ∪ ar_int)⁺ ⨾ sb^? ∪ sb.
 Proof.
-unfold imm_hb.hb.
-rewrite (dom_r (wf_swD WF)).
-rewrite (sw_in_ar WF); relsf.
-arewrite ((sb ∪ ((sb^? ⨾ ⦗W⦘ ⨾ ar⁺ ⨾ (rmw ⨾ sb^?)^?) ⨾ ⦗F ∩₁ Acq ∪₁ R ∩₁ Acq⦘
-      ∪ sb ⨾ ⦗F ∩₁ Acq ∪₁ R ∩₁ Acq⦘)) ⊆ sb ∪ sb^? ⨾ ⦗W⦘ ⨾ ar⁺ ⨾ (rmw ⨾ sb^?)^? ⨾ ⦗FR ∩₁ Acq⦘).
-by basic_solver 21.
-rewrite path_union.
-generalize (@sb_trans G); ins; relsf; unionL.
-by rewrite <- ct_step; unfold ar, imm_ppo.ar_int, imm_bob.bob, imm_bob.fwbob; mode_solver 21.
-rewrite ct_seq_swap, !seqA.
-rewrite ct_rotl, !seqA.
-arewrite ((rmw ⨾ sb^?)^? ⨾ ⦗F ∩₁ Acq ∪₁ R ∩₁ Acq⦘ ⨾ sb^? ⨾ ⦗W⦘ ⊆ ar^?).
-{ case_refl (rmw ⨾ sb^?).
-  - arewrite (⦗F ∩₁ Acq ∪₁ R ∩₁ Acq⦘ ⊆ ⦗R ∩₁ Acq⦘ ∪ ⦗F ∩₁ Acq/Rel⦘) by mode_solver.
-    unfold ar, imm_ppo.ar_int, imm_bob.bob, imm_bob.fwbob; basic_solver 15.
-  - unfold ar, imm_ppo.ar_int, imm_ppo.ppo.
-    rewrite <- ct_step.
-    arewrite_id ⦗F ∩₁ Acq ∪₁ R ∩₁ Acq⦘; relsf.
-    rewrite (dom_l (wf_rmwD WF)) at 1.
-    rewrite (dom_l (wf_rmwD WF)), R_ex_in_R at 1.
-    rewrite (rmw_in_sb WF).
-    generalize (@sb_trans G); basic_solver 21. }
-arewrite ((rmw ⨾ sb^?)^? ⨾ ⦗F ∩₁ Acq ∪₁ R ∩₁ Acq⦘ ⨾ sb^? ⊆ sb^?).
-by rewrite (rmw_in_sb WF); basic_solver.
-arewrite (sb^? ⨾ ⦗F ∩₁ Sc⦘ ⊆ ar^?).
-by unfold ar, imm_ppo.ar_int, imm_bob.bob, imm_bob.fwbob; mode_solver 21.
-arewrite (⦗F ∩₁ Sc⦘ ⨾ sb^? ⨾ ⦗W⦘ ⊆ ar^?).
-by unfold ar, imm_ppo.ar_int, imm_bob.bob, imm_bob.fwbob; mode_solver 21.
+rewrite (sw_in_ar1 WF).
+remember (rfe ∪ ar_int) as ax.
+relsf; unionL; [| | basic_solver 21].
+- arewrite ((⦗F ∩₁ Rel⦘ ⨾ sb) ⊆ ax).
+{ desf. 
+rewrite <- bob_in_ar_int, <- fwbob_in_bob.
+unfold imm_common.fwbob.
+mode_solver 12. }
+arewrite (ax ⊆ ax^*) at 1.
 relsf.
+- rewrite crE; relsf; unionL.
+basic_solver 12.
+arewrite (⦗W ∩₁ Rel⦘ ⨾ sb ∩ same_loc ⨾ ⦗W⦘ ⊆ ax).
+{ desf.
+rewrite <- bob_in_ar_int, <- fwbob_in_bob.
+unfold imm_common.fwbob.
+basic_solver 12. }
+arewrite (ax ⊆ ax^*) at 1.
+relsf.
+Qed.
+
+Lemma f_sc_hb_f_sc_in_ar WF :
+  ⦗F ∩₁ Sc⦘ ⨾ hb ⨾ ⦗F ∩₁ Sc⦘ ⊆ (rfe ∪ ar_int)⁺.
+Proof.
+
+  unfold imm_hb.hb.
+rewrite (dom_l (wf_swD WF)).
+  rewrite (sw_in_ar WF).
+remember (rfe ∪ ar_int) as ax.
+rewrite seq_union_r.
+arewrite (⦗FW ∩₁ Rel⦘ ⨾ sb ⊆ sb).
+
+
+
+  rewrite unionC.
+  rewrite unionA.
+  arewrite (sb ∪ sb ⊆ sb).
+  rewrite unionC.
+  rewrite path_union.
+  (* arewrite ((sb ∪ ((sb^? ⨾ ⦗W⦘ ⨾ ar⁺ ⨾ (rmw ⨾ (sb ∩ same_loc)^?)^?) ⨾ ⦗F ∩₁ Acq ∪₁ R ∩₁ Acq⦘ *)
+  (*               ∪ sb ⨾ ⦗F ∩₁ Acq ∪₁ R ∩₁ Acq⦘)) ⊆ *)
+  (*           sb ∪ sb^? ⨾ ⦗W⦘ ⨾ ar⁺ ⨾ (rmw ⨾ sb^?)^? ⨾ ⦗FR ∩₁ Acq⦘). *)
+  (* { by basic_solver 21. } *)
+  generalize (@sb_trans G); ins; relsf; unionL.
+  { desf; rewrite <- ct_step; unfold imm_common.ar_int, imm_common.bob, imm_common.fwbob.
+    mode_solver 21. }
+  rewrite ct_seq_swap.
+rewrite !seqA.
+relsf.
+  rewrite ct_rotl, !seqA.
+
+assert (sb^? ⨾ ⦗F ∩₁ Rel ∪₁ W ∩₁ Rel⦘ ⊆ ax^?) as BB.
+{ desf.
+rewrite <- bob_in_ar_int, <- fwbob_in_bob.
+unfold imm_common.fwbob.
+mode_solver 12. }
+
+sin_rewrite !BB.
+
+arewrite (sb^? ⨾ ⦗F ∩₁ Sc⦘ ⊆ ax^?).
+{ desf.
+rewrite <- bob_in_ar_int, <- fwbob_in_bob.
+unfold imm_common.fwbob.
+mode_solver 12. }
+
+rels.
+basic_solver.
 Qed.
 
 Lemma acyc_ext_helper WF :
