src/imm/imm_s_ppo.v
@@ -1,0 +1,277 @@
+(******************************************************************************)
+(** * Definition of s_IMM PPO  *)
+(******************************************************************************)
+
+Require Import Classical Peano_dec.
+From hahn Require Import Hahn.
+
+Require Import Events.
+Require Import Execution.
+Require Import Execution_eco.
+Require Import imm_bob.
+
+Set Implicit Arguments.
+Remove Hints plus_n_O.
+
+Section IMM_S_PPO.
+
+Variable G : execution.
+
+Notation "'E'" := G.(acts_set).
+Notation "'sb'" := G.(sb).
+Notation "'rf'" := G.(rf).
+Notation "'co'" := G.(co).
+Notation "'rmw'" := G.(rmw).
+Notation "'data'" := G.(data).
+Notation "'addr'" := G.(addr).
+Notation "'ctrl'" := G.(ctrl).
+Notation "'rmw_dep'" := G.(rmw_dep).
+
+Notation "'fr'" := G.(fr).
+Notation "'eco'" := G.(eco).
+Notation "'coe'" := G.(coe).
+Notation "'coi'" := G.(coi).
+Notation "'deps'" := G.(deps).
+Notation "'rfi'" := G.(rfi).
+Notation "'rfe'" := G.(rfe).
+Notation "'detour'" := G.(detour).
+
+Notation "'lab'" := G.(lab).
+Notation "'loc'" := (loc lab).
+Notation "'val'" := (val lab).
+Notation "'mod'" := (mod lab).
+Notation "'same_loc'" := (same_loc lab).
+
+Notation "'R'" := (fun a => is_true (is_r lab a)).
+Notation "'W'" := (fun a => is_true (is_w lab a)).
+Notation "'F'" := (fun a => is_true (is_f lab a)).
+Notation "'RW'" := (R ∪₁ W).
+Notation "'FR'" := (F ∪₁ R).
+Notation "'FW'" := (F ∪₁ W).
+Notation "'R_ex'" := (fun a => is_true (R_ex lab a)).
+Notation "'W_ex'" := (W_ex G).
+Notation "'W_ex_acq'" := (W_ex ∩₁ (fun a => is_true (is_xacq lab a))).
+
+Notation "'Pln'" := (fun a => is_true (is_only_pln lab a)).
+Notation "'Rlx'" := (fun a => is_true (is_rlx lab a)).
+Notation "'Rel'" := (fun a => is_true (is_rel lab a)).
+Notation "'Acq'" := (fun a => is_true (is_acq lab a)).
+Notation "'Acqrel'" := (fun a => is_true (is_acqrel lab a)).
+Notation "'Acq/Rel'" := (fun a => is_true (is_ra lab a)).
+Notation "'Sc'" := (fun a => is_true (is_sc lab a)).
+
+Notation "'fwbob'" := (fwbob G).
+Notation "'bob'" := (bob G).
+
+(******************************************************************************)
+(** ** Derived relations  *)
+(******************************************************************************)
+
+Definition ppo := ⦗R⦘ ⨾ (data ∪ ctrl ∪ addr ⨾ sb^? ∪ rfi ∪
+                              rmw ;; ((sb ∩ same_loc) ⨾ ⦗W⦘)^? ∪ rmw_dep ;; sb^?)⁺ ⨾ ⦗W⦘.
+
+Definition ar_int := bob ∪ ppo ∪ detour ∪ ⦗W_ex_acq⦘ ⨾ sb ⨾ ⦗W⦘ 
+                     ∪ ⦗W_ex⦘ ⨾ rfi ⨾ ⦗R∩₁Acq⦘.
+
+Implicit Type WF : Wf G.
+Implicit Type COMP : complete G.
+
+Lemma ppo_in_sb WF: ppo ⊆ sb.
+Proof using.
+unfold ppo.
+rewrite (addr_in_sb WF), (data_in_sb WF), (ctrl_in_sb WF).
+rewrite (rmw_dep_in_sb WF).
+arewrite (rfi ⊆ sb).
+rewrite WF.(rmw_in_sb).
+rewrite inclusion_seq_eqv_l, inclusion_seq_eqv_r.
+assert (sb⁺ ⊆ sb) as AA.
+{ generalize (@sb_trans G). ins. relsf. }
+etransitivity.
+2: by apply AA.
+apply clos_trans_mori.
+generalize (@sb_trans G); ins; relsf.
+generalize (@sb_trans G). basic_solver 10.
+Qed.
+
+Lemma rmw_in_ppo WF : rmw ⊆ ppo.
+Proof using.
+unfold ppo; rewrite (wf_rmwD WF) at 1.
+rewrite R_ex_in_R at 1.
+rewrite <- ct_step.
+basic_solver 10.
+Qed.
+
+(* Lemma rmw_sb_W_in_ppo WF : rmw ⨾ sb ⨾ ⦗W⦘ ⊆ ppo. *)
+(* Proof. *)
+(* unfold ppo; rewrite (wf_rmwD WF). *)
+(* rewrite (dom_l (wf_rmwD WF)), R_ex_in_R at 1. *)
+(* rewrite (rmw_in_sb WF) at 1. *)
+(* rewrite <- ct_step. *)
+(* generalize (@sb_trans G). *)
+(* basic_solver 12. *)
+(* Qed. *)
+
+Lemma data_in_ppo WF : data ⊆ ppo.
+Proof using.
+unfold ppo; rewrite (wf_dataD WF) at 1.
+hahn_frame; econs; basic_solver 12.
+Qed.
+
+(* Lemma R_ex_sb_in_ppo WF : ⦗R_ex⦘ ⨾ sb ⨾ ⦗W⦘ ⊆ ppo. *)
+(* Proof using. *)
+(*   arewrite (⦗R_ex⦘ ⊆ ⦗R⦘ ;; ⦗R_ex⦘) by type_solver. *)
+(*   unfold ppo. hahn_frame. rewrite <- ct_step. eauto with hahn. *)
+(* Qed. *)
+
+(* Lemma rmw_sb_cr_W_in_ppo WF : rmw ⨾ sb^? ⨾ ⦗W⦘ ⊆ ppo. *)
+(* Proof using. *)
+(*   rewrite crE. rewrite seq_union_l, seq_union_r, seq_id_l. *)
+(*   rewrite WF.(rmw_sb_W_in_ppo). *)
+(*   rewrite WF.(rmw_in_ppo). eauto with hahn hahn_full. *)
+(* Qed. *)
+
+Lemma wf_ppoE WF : ppo ≡ ⦗E⦘ ⨾ ppo ⨾ ⦗E⦘.
+Proof using.
+split; [|basic_solver].
+unfold ppo.
+rewrite !seqA, seq_eqvC.
+hahn_frame.
+seq_rewrite seq_eqvC.
+rewrite !seqA.
+hahn_frame.
+rewrite <- inclusion_ct_seq_eqv_r, <- inclusion_ct_seq_eqv_l.
+apply inclusion_t_t.
+unfold Execution.rfi.
+rewrite (wf_rfE WF), (wf_dataE WF), (wf_rmw_depE WF) at 1.
+rewrite (wf_addrE WF), (wf_ctrlE WF), (wf_rmwE WF) at 1.
+rewrite wf_sbE at 1 2 3 4.
+basic_solver 21.
+Qed.
+
+Lemma wf_ar_intE WF : ar_int ≡ ⦗E⦘ ⨾ ar_int ⨾ ⦗E⦘.
+Proof using.
+split; [|basic_solver].
+unfold ar_int.
+rewrite (wf_bobE WF), (wf_ppoE WF) at 1.
+rewrite (wf_detourE WF), (@wf_sbE G), (wf_rfiE WF).
+basic_solver 42.
+Qed.
+
+Lemma wf_ppoD: ppo ≡ ⦗R⦘ ⨾ ppo ⨾ ⦗W⦘.
+Proof using.
+split; [|basic_solver].
+unfold ppo; basic_solver.
+Qed.
+
+Lemma fwbob_ppo WF: fwbob ⨾ ppo ⊆ fwbob.
+Proof using.
+rewrite wf_ppoD, (ppo_in_sb WF).
+sin_rewrite fwbob_r_sb.
+basic_solver.
+Qed.
+
+Lemma bob_ppo WF: bob ⨾ ppo ⊆ bob.
+Proof using.
+rewrite wf_ppoD, (ppo_in_sb WF).
+sin_rewrite bob_r_sb.
+basic_solver.
+Qed.
+
+Lemma ar_int_in_sb WF: ar_int ⊆ sb.
+Proof using.
+unfold ar_int.
+rewrite bob_in_sb.
+rewrite (ppo_in_sb WF).
+arewrite (detour ⊆ sb).
+arewrite (rfi ⊆ sb).
+basic_solver 21.
+Qed.
+
+Lemma ppo_rfi_ppo : ppo ⨾ rfi ⨾ ppo ⊆ ppo.
+Proof using.
+unfold ppo.
+rewrite !seqA.
+arewrite_id ⦗W⦘ at 2.
+arewrite_id ⦗R⦘ at 2.
+arewrite (rfi ⊆ (data ∪ ctrl ∪ addr ⨾ sb^? ∪ rfi ∪ rmw ⨾ (sb ∩ same_loc ⨾ ⦗W⦘)^? ∪ rmw_dep ⨾ sb^?)＊) at 2.
+rewrite inclusion_t_rt at 1.
+relsf.
+Qed.
+
+Lemma deps_rfi_in_ppo : ⦗R⦘ ⨾ (deps ∪ rfi)⁺ ⨾ ⦗W⦘ ⊆ ppo.
+Proof using.
+  unfold ppo, Execution.deps.
+  hahn_frame.
+  apply inclusion_t_t; basic_solver 21.
+Qed.
+
+(* Lemma ppo_alt WF  *)
+(*   (RMW_DEPS : rmw ⊆ deps) *)
+(*   (DEPS_RMW_FAIL : rmw_dep ⨾ sb ⊆ ctrl) :  *)
+(*   ppo ≡ ⦗R⦘ ⨾ (data ∪ ctrl ∪ addr ⨾ sb^? ∪ rfi)⁺ ⨾ ⦗W⦘. *)
+(* Proof using. *)
+(*   unfold ppo. *)
+(* Admitted. *)
+
+(* generalize (@sb_trans G); ins. *)
+(* unfold ppo. *)
+(* split. *)
+(* 2: by hahn_frame; apply inclusion_t_t; basic_solver 12. *)
+(* rewrite RMW_DEPS; unfold Execution.deps. *)
+(* rewrite path_ut_first; relsf; unionL. *)
+(* by hahn_frame; apply inclusion_t_t; basic_solver 12. *)
+(* arewrite ((data ∪ ctrl ∪ addr ⨾ sb^? ∪ rfi ∪ (data ∪ addr ∪ ctrl) ∪ rmw_dep ⨾ sb^?) ⊆ sb). *)
+(* { rewrite (data_in_sb WF), (addr_in_sb WF), (ctrl_in_sb WF). *)
+(*   arewrite (rfi ⊆ sb). *)
+(*   rewrite (rmw_dep_in_sb WF). *)
+(*   relsf. } *)
+(* relsf. *)
+(* rewrite (dom_r (wf_rmw_depD WF)), !seqA. *)
+(* rewrite (crE sb) at 2; relsf; unionL. *)
+(* by rewrite R_ex_in_R; type_solver. *)
+(* hahn_frame. *)
+(* sin_rewrite RMW_CTRL_FAIL. *)
+(* rewrite DEPS_RMW_FAIL. *)
+(* rewrite ct_end. *)
+(* apply inclusion_seq_mon; [apply inclusion_rt_rt|]; basic_solver 42. *)
+(* Qed. *)
+
+Lemma bob_in_ar_int : bob ⊆ ar_int.
+Proof using. unfold ar_int. basic_solver 10. Qed.
+
+Lemma ppo_in_ar_int : ppo ⊆ ar_int.
+Proof using. unfold ar_int. basic_solver 10. Qed.
+
+Lemma detour_in_ar_int : detour ⊆ ar_int.
+Proof using. unfold ar_int. basic_solver. Qed.
+
+Lemma w_ex_acq_sb_w_in_ar_int : ⦗W_ex_acq⦘ ⨾ sb ⨾ ⦗W⦘ ⊆ ar_int.
+Proof using. unfold ar_int. basic_solver 10. Qed.
+
+Lemma bob_ppo_W_sb WF :
+  (bob ∪ ppo ∪ ⦗W_ex_acq⦘ ⨾ sb ⨾ ⦗W⦘)⁺ ⊆ ppo ∪ ppo ^? ;; (bob ∪ ⦗W_ex_acq⦘ ⨾ sb ⨾ ⦗W⦘)^+.
+Proof using.
+arewrite (bob ∪ ppo ∪ ⦗W_ex_acq⦘ ⨾ sb ⨾ ⦗W⦘ ⊆
+         (bob ∪ ⦗W_ex_acq⦘ ⨾ sb ⨾ ⦗W⦘) ∪ ppo).
+basic_solver 12.
+apply ct_ind_left with (P:= fun r =>  r).
+by auto with hahn.
+- arewrite(bob ⊆ (bob ∪ ⦗W_ex_acq⦘ ⨾ sb ⨾ ⦗W⦘)⁺).
+  arewrite(⦗W_ex_acq⦘ ⨾ sb ⨾ ⦗W⦘ ⊆ (bob ∪ ⦗W_ex_acq⦘ ⨾ sb ⨾ ⦗W⦘)⁺) at 2.
+  basic_solver 12.
+- intros k H. rewrite H; clear k H; rewrite crE; relsf; unionL.
++ rewrite (bob_ppo WF). 
+  arewrite(bob ⊆ (bob ∪ ⦗W_ex_acq⦘ ⨾ sb ⨾ ⦗W⦘)⁺).
+  basic_solver.
++ rewrite (wf_ppoD) at 1. type_solver.
++ rewrite (wf_ppoD) at 1 2. type_solver.
++ arewrite(bob ⊆ (bob ∪ ⦗W_ex_acq⦘ ⨾ sb ⨾ ⦗W⦘)^*); relsf.
++ sin_rewrite (bob_ppo WF). 
+  arewrite(bob ⊆ (bob ∪ ⦗W_ex_acq⦘ ⨾ sb ⨾ ⦗W⦘)^*); relsf.
++ arewrite(⦗W_ex_acq⦘ ⨾ sb ⨾ ⦗W⦘ ⊆ (bob ∪ ⦗W_ex_acq⦘ ⨾ sb ⨾ ⦗W⦘)^*) at 1; relsf.
++ rewrite (wf_ppoD) at 1. type_solver.
++ basic_solver 12.
++ rewrite (wf_ppoD) at 1 2. type_solver.
+Qed.
+
+End IMM_S_PPO.
